compiler/backend/proofs/source_to_sourceIcingProofsScript.sml
@@ -1,0 +1,270 @@
+(*
+  Correctness proofs for floating-point optimizations
+*)
+
+open source_to_sourceIcingTheory fpOptPropsTheory semanticPrimitivesTheory evaluateTheory
+     terminationTheory;
+open preamble;
+
+val _ = new_theory "source_to_sourceIcingProofs";
+
+Theorem no_match_word_cond:
+  ! w e s1 s2.
+    matchesFPcexp (Word w) e s1 = SOME s2 ==> F
+Proof
+  rpt strip_tac
+  \\ Cases_on `e` \\ fs[matchesFPcexp_def]
+  \\ rename [`App op l`]
+  \\ Cases_on `l` \\ fs[matchesFPcexp_def]
+  \\ Cases_on `t` \\ fs[matchesFPcexp_def]
+QED
+
+Theorem no_match_var_cond:
+  ! n e s1 s2.
+    matchesFPcexp (Var n) e s1 = SOME s2 ==> F
+Proof
+  rpt strip_tac
+  \\ Cases_on `e` \\ fs[matchesFPcexp_def]
+  \\ rename [`App op l`]
+  \\ Cases_on `l` \\ fs[matchesFPcexp_def]
+  \\ Cases_on `t` \\ fs[matchesFPcexp_def]
+QED
+
+Theorem matchExpr_preserving:
+  ! p.
+    (! e s1 s2.
+     matchesFPexp p e s1 = SOME s2 ==>
+      substMonotone s1 s2)
+  /\
+    (! ce s1 s2.
+      matchesFPcexp p ce s1 = SOME s2 ==>
+      substMonotone s1 s2)
+Proof
+  Induct_on `p`
+  \\ simp[no_match_word_cond, no_match_var_cond]
+  \\ rpt gen_tac \\ TRY conj_tac
+  \\ simp[Once matchesFPexp_def, option_case_eq]
+  \\ simp[Once matchesFPcexp_def]
+  \\ TRY (fs[substMonotone_def] \\ rpt strip_tac \\ imp_res_tac substLookup_substUpdate \\ rveq \\ fs[] \\ NO_TAC)
+  \\ rpt gen_tac
+  \\ rpt (TOP_CASE_TAC \\ fs[substMonotone_def]) \\ rpt strip_tac \\ fs[substMonotone_def]
+  \\ rpt res_tac
+QED
+
+Theorem appFPexp_weakening:
+  ! p.
+    (! e s1 s2.
+      substMonotone s1 s2 /\
+      appFPexp p s1 = SOME e ==>
+      appFPexp p s2 = SOME e) /\
+    (! ce s1 s2.
+      substMonotone s1 s2 /\
+      appFPcexp p s1 = SOME ce ==>
+      appFPcexp p s2 = SOME ce)
+Proof
+  Induct_on `p`
+  \\ rpt strip_tac \\ fs[]
+  \\ fs[appFPexp_def, appFPcexp_def, pair_case_eq, option_case_eq, substMonotone_def]
+  \\ res_tac \\ fs[]
+QED
+
+val exprSolve_tac =
+  (let
+    val thms = CONJ_LIST 2 (SIMP_RULE std_ss [FORALL_AND_THM] appFPexp_weakening)
+  in
+  (irule (hd thms) ORELSE irule (hd (tl thms)))
+  end)
+  \\ asm_exists_tac \\ fs[substMonotone_def]
+  \\ rpt strip_tac
+  \\ imp_res_tac matchExpr_preserving \\ fs[substMonotone_def];
+
+Theorem subst_pat_is_exp:
+  ! p.
+    (! e s1 s2.
+      matchesFPexp p e s1 = SOME s2 ==>
+      appFPexp p s2 = SOME e) /\
+    (! ce s1 s2.
+      matchesFPcexp p ce s1 = SOME s2 ==>
+      appFPcexp p s2 = SOME ce)
+Proof
+  Induct_on `p` \\ rpt gen_tac \\ conj_tac
+  \\ rpt gen_tac
+  \\ simp[Once matchesFPexp_def]
+  \\ simp[Once matchesFPcexp_def, option_case_eq]
+  \\ rpt (TOP_CASE_TAC \\ fs[]) \\ rpt strip_tac \\ rveq
+  \\ fs[Once appFPexp_def, Once appFPcexp_def]
+  \\ TRY (imp_res_tac substLookup_substUpdate \\ fs[])
+  \\ res_tac \\ fs[]
+  \\ rpt conj_tac \\ exprSolve_tac
+QED
+
+local
+  val eval_goal =
+    ``\ (ffi:'ffi state) env el.
+        ! res ffi2 opt.
+          evaluate ffi env el = (ffi2, res) ==>
+          evaluate (ffi with fp_rws := ffi.fp_rws ++ [opt]) env el =
+            (ffi2 with fp_rws := ffi2.fp_rws ++ [opt], res)``
+  val eval_match_goal =
+    ``\ (ffi:'ffi state) env v pl err_v.
+        ! res ffi2 opt.
+          evaluate_match ffi env v pl err_v = (ffi2, res) ==>
+          evaluate_match (ffi with fp_rws := ffi.fp_rws ++ [opt]) env v pl err_v =
+            (ffi2 with fp_rws := ffi2.fp_rws ++ [opt], res)``
+  val indThm = terminationTheory.evaluate_ind
+    |> ISPEC eval_goal |> SPEC eval_match_goal
+in
+Theorem evaluate_fp_rws_append:
+  (! (ffi:'ffi state) env el.
+    ^eval_goal ffi env el) /\
+  (! (ffi:'ffi state) env v pl err_v.
+    ^eval_match_goal ffi env v pl err_v)
+Proof
+  match_mp_tac indThm
+  \\ rpt strip_tac \\ fs[evaluate_def] \\ rpt strip_tac \\ rveq \\ fs[]
+  \\ qpat_x_assum `_ = (_, _)` mp_tac
+  \\ TRY (rpt (TOP_CASE_TAC \\ fs[]) \\ NO_TAC)
+  \\ TRY (rpt (TOP_CASE_TAC \\ fs[]) \\ rpt strip_tac \\ rveq
+          \\ fs[state_component_equality] \\ NO_TAC)
+  \\ ntac 2 (TOP_CASE_TAC \\ fs[])
+  \\ Cases_on `op = Opapp` \\ fs[]
+  >- (rveq \\ rpt (TOP_CASE_TAC \\ fs[dec_clock_def]))
+  \\ ntac 3 (TOP_CASE_TAC \\ fs[])
+  \\ Cases_on `isFpOp op` \\ fs[]
+  >- (rpt strip_tac \\ rveq \\ fs[state_component_equality, list_result_def, shift_fp_opts_def]
+      \\ Cases_on `isFpBool op` \\ fs[]
+      >- (Cases_on `do_fprw r (q.fp_opts 0) q.fp_rws` \\ fs[]
+          >- (`do_fprw r (q.fp_opts 0) (q.fp_rws ++ [opt]) = NONE` by (cheat)
+              \\ fs[])
+          \\ `do_fprw r (q.fp_opts 0) (q.fp_rws ++ [opt]) = SOME x` by (cheat)
+          \\ fs[])
+      \\ Cases_on `do_fprw r (q.fp_opts 0) q.fp_rws` \\ fs[]
+      >- (`do_fprw r (q.fp_opts 0) (q.fp_rws ++ [opt]) = NONE` by (cheat)
+          \\ fs[])
+      \\ `do_fprw r (q.fp_opts 0) (q.fp_rws ++ [opt]) = SOME x` by (cheat)
+      \\ fs[])
+  \\ rpt strip_tac \\ fs[state_component_equality]
+QED
+end
+
+Theorem fp_add_comm_cases:
+  ! e.
+    (? e1 e2.
+      e = (App (FP_bop FP_Add) [e1; e2]) /\
+      rewriteFPexp [fp_add_comm] (App (FP_bop FP_Add) [e1; e2]) =
+        App (FP_bop FP_Add) [e2; e1]) \/
+    (rewriteFPexp [fp_add_comm] e = e)
+Proof
+  rpt gen_tac \\ fs[rewriteFPexp_def, fp_add_comm_def, matchesFPexp_def]
+  \\ Cases_on `e` \\ fs[]
+  \\ rename1 `App op els`
+  \\ Cases_on `op` \\ fs[]
+  \\ Cases_on `f` \\ fs[] \\ EVAL_TAC
+QED
+
+Theorem ffi_eq_fp_opts[local]:
+  ffi with <| fp_rws := rws |> =
+    ffi with <| fp_rws := rws; fp_opts := ffi.fp_opts |>
+Proof
+  fs[state_component_equality]
+QED
+
+val theTheorem
+SIMP_RULE std_ss [Once test] evaluate_fp_rws_append
+  |> CONJ_LIST 2
+  |> map (Q.SPEC `ffi with fp_opts:= ffi.fp_opts`)
+
+local
+  val eval_goal =
+    ``\ (ffi1:'ffi state) env el.
+        ! ffi2 m n k r f.
+          evaluate ffi1 env el = (ffi2, r) /\
+          (!m. m >= n ==> ffi2.fp_opts (m - n) = ffi1.fp_opts m) /\
+          k >= n /\
+          (!m. m >= k ==> f m = ffi1.fp_opts m) ==>
+          ? ffi3.
+          evaluate (ffi1 with fp_opts := f) env el = (ffi3, r) /\
+          (!m. m >= n ==> ffi3.fp_opts m = f m)``
+  val eval_match_goal =
+    ``\ (ffi1:'ffi state) env v pl err_v.
+        ! ffi2 m n k r f.
+          evaluate_match ffi1 env v pl err_v = (ffi2, r) ==>
+          (!m. m >= n ==> ffi2.fp_opts (m - n) = ffi1.fp_opts m) /\
+          k >= n /\
+          (!m. m >= k ==> f m = ffi1.fp_opts m) ==>
+          ? ffi3.
+          evaluate_match (ffi1 with fp_opts := f) env v pl err_v = (ffi3, r) /\
+          (!m. m >= n ==> ffi3.fp_opts m = f m)``
+  val indThm = terminationTheory.evaluate_ind
+    |> ISPEC eval_goal |> SPEC eval_match_goal
+  val choice_det_thm =
+    SIMP_RULE std_ss [] evaluatePropsTheory.evaluate_fp_opt_choice_det;
+in
+Theorem evaluate_ignore_higher_rw:
+  (! (ffi:'ffi state) env el.
+    ^eval_goal ffi env el) /\
+  (! (ffi:'ffi state) env v pl err_v.
+    ^eval_match_goal ffi env v pl err_v)
+Proof
+  match_mp_tac indThm \\ rpt strip_tac \\ fs[evaluate_def]
+  >- (rpt strip_tac
+      \\ qpat_x_assum `_ = (_, _)` mp_tac
+      \\ ntac 2 (TOP_CASE_TAC \\ fs[])
+      >- (ntac 2 (TOP_CASE_TAC \\ fs[])
+          >- (rpt strip_tac \\ rveq \\ fs[]
+              \\ imp_res_tac choice_det_thm
+              \\ res_tac \\ fs[]
+QED
+
+local
+  val fp_rws_append_comm =
+    SIMP_RULE std_ss [Once ffi_eq_fp_opts] evaluate_fp_rws_append
+    |> CONJ_LIST 2
+    |> map (SPEC_ALL) |> map (GEN ``(opt:fp_pat #fp_pat)``)
+    |> map (Q.SPEC `fp_add_comm`) |> map GEN_ALL
+    |> LIST_CONJ;
+  val loc_eval_fp_opt_choice_det =
+    SIMP_RULE std_ss [] evaluatePropsTheory.evaluate_fp_opt_choice_det
+    |> CONJ_LIST 2 |> hd;
+in
+Theorem fp_add_comm_correct:
+  ! (ffi1 ffi2:'ffi state) env e res.
+    evaluate ffi1 env [rewriteFPexp [fp_add_comm] e] = (ffi2, Rval res) ==>
+    ? (fp_opts:num -> rewrite_app list).
+      evaluate
+        (ffi1 with <| fp_rws := ffi1.fp_rws ++ [fp_add_comm]; fp_opts := fp_opts |>)
+        env [e] =
+        (ffi2 with <| fp_rws := ffi2.fp_rws ++ [fp_add_comm] |>, Rval res)
+Proof
+  rpt strip_tac
+  \\ qspec_then `e` assume_tac fp_add_comm_cases
+  \\ fs[]
+  >- (
+    fs[evaluate_def] \\ rveq
+    \\ qpat_x_assum `_ = (_, _)` mp_tac
+    \\ rename [`evaluate ffi1 env [e1]`]
+    \\ Cases_on `evaluate ffi1 env [e1]` \\ fs[]
+    \\ rename [`evaluate ffi1 env [e1] = (ffi2, r)`] \\ Cases_on `r` \\ fs[]
+    \\ rename [`evaluate ffi2 env [e2]`]
+    \\ Cases_on `evaluate ffi2 env [e2]` \\ fs[]
+    \\ rename [`evaluate ffi2 env [e2] = (ffi3, r)`] \\ Cases_on `r` \\ fs[]
+    \\ ntac 3 (TOP_CASE_TAC \\ fs[])
+    \\ fs[astTheory.isFpOp_def, astTheory.isFpBool_def]
+    \\ rpt strip_tac \\ rveq
+    \\ imp_res_tac loc_eval_fp_opt_choice_det
+    \\ rename [`!m. m >= n1 ==> ffi2.fp_opts (m - n1) = ffi1.fp_opts m`,
+               `!m. m >= n2 ==> ffi3.fp_opts (m - n2) = ffi2.fp_opts m`]
+    \\ qexists_tac
+        `\x.
+          if (x = (n1 + n2))
+          then [RewriteApp Here (LENGTH ffi1.fp_rws)] ++ ffi1.fp_opts x
+          else ffi1.fp_opts x`
+    \\ qmatch_abbrev_tac `evaluate ffi1upd env [e2]`
+    \\ cheat (* qexists_tac `` fp_opts should 1. do decisions of ffi1, then ffi2, then ffi3 + comm *)
+    )
+  \\ fs[]
+  \\ qexists_tac `ffi1.fp_opts` \\ fs[state_component_equality]
+  \\ imp_res_tac fp_rws_append_comm
+QED
+
+val _ = export_theory ();
