compiler/backend/source_to_sourceIcingScript.sml
@@ -1,0 +1,148 @@
+(*
+  Source to source pass, applying Icing optimizations
+*)
+
+open semanticPrimitivesTheory evaluateTheory;
+open terminationTheory;
+
+open preamble;
+
+val _ = new_theory "source_to_sourceIcing";
+
+val _  = monadsyntax.enable_monadsyntax();
+val _ = List.app monadsyntax.enable_monad ["option"];
+
+(* matching function for expressions *)
+Definition matchesFPexp_def:
+  matchesFPexp p e s =
+    case (p, e) of
+    | Word w1, Lit (Word64 w2) =>
+      if (w1 = w2) then SOME s else NONE
+    | Var n, _ =>
+      (case substLookup s n of
+      | SOME e1 => if e1 = e  then SOME s else NONE
+      | NONE => substUpdate n e s)
+    | Unop op1 p, App (FP_uop op2) [e1] =>
+      (if (op1 = op2)
+      then matchesFPexp p e1 s
+      else NONE)
+    | Binop op1 p1 p2, App (FP_bop op2) [e1;e2] =>
+      (if (op1 = op2)
+      then do
+        s1 <- matchesFPexp p1 e1 s;
+        matchesFPexp p2 e2 s1;
+        od
+      else NONE)
+    | Terop op1 p1 p2 p3, App (FP_top op2) [e1;e2;e3] =>
+      (if (op1 = op2)
+      then do
+        s1 <- matchesFPexp p1 e1 s;
+        s2 <- matchesFPexp p2 e2 s1;
+        matchesFPexp p3 e3 s2;
+        od
+      else NONE)
+  (*
+    | Scope sc1 p, App (FP_sc sc2) [e1] =>
+      (if sc1 = sc2
+      then matchesFPexp p e1 s
+      else NONE) *)
+    | _, _ => NONE
+Termination
+  wf_rel_tac (`measure \ (x,y,z). fp_pat_size x`)
+End
+
+Definition matchesFPcexp_def:
+  matchesFPcexp p e s =
+    case p, e of
+    | Pred p1 p, App (FP_pred p2) [e1] =>
+      (if (p1 = p2) then matchesFPexp p e1 s else NONE)
+    | Cmp cmp1 p1 p2, App (FP_cmp cmp2) [e1; e2] =>
+      (if (cmp1 = cmp2)
+      then do
+        s1 <- matchesFPexp p1 e1 s;
+        matchesFPexp p2 e2 s1;
+        od
+      else NONE)
+    (*
+    | Scope sc1 p, App (FP_sc sc2) [e1] =>
+      (if sc1 = sc2 then matchesFPcexp p e1 s else NONE) *)
+    | _, _ => NONE
+End
+
+(* Instantiate a given fp_pattern with a substitution into an expression *)
+Definition appFPexp_def:
+  appFPexp (Word w) s = SOME (Lit (Word64 w)) /\
+  appFPexp (Var n) s = substLookup s n /\
+  appFPexp (Unop u p) s = (do e <- appFPexp p s; return (App (FP_uop u) [e]); od) /\
+  appFPexp (Binop op p1 p2) s =
+    (do
+      e1 <- appFPexp p1 s;
+      e2 <- appFPexp p2 s;
+      return (App (FP_bop op) [e1; e2]);
+    od) /\
+  appFPexp (Terop op p1 p2 p3) s =
+    (do
+      e1 <- appFPexp p1 s;
+      e2 <- appFPexp p2 s;
+      e3 <- appFPexp p3 s;
+      return (App (FP_top op) [e1; e2; e3]);
+    od) /\
+  (*
+  appFPexp (Scope sc p) s =
+    (do
+      e <- appFPexp p s;
+      return (App (FP_sc sc) [e]);
+    od) /\ *)
+  appFPexp _ _ = NONE
+End
+
+Definition appFPcexp_def:
+  appFPcexp (Pred pr p) s =
+    (do
+      e <- appFPexp p s;
+      return (App (FP_pred pr) [e]);
+    od) /\
+  appFPcexp (Cmp cmp p1 p2) s =
+    (do
+      e1 <- appFPexp p1 s;
+      e2 <- appFPexp p2 s;
+      return (App (FP_cmp cmp) [e1; e2]);
+    od) /\
+  (*
+  appFPcexp (Scope sc p) s =
+    (do
+      e <- appFPcexp p s;
+      return (App (FP_sc sc) [e]);
+    od) /\ *)
+  appFPcexp _ _ = NONE
+End
+
+(* rewriteExp: Recursive, expression rewriting function applying all rewrites that match.
+  A non-matching rewrite is silently ignored *)
+Definition rewriteFPexp_def:
+  rewriteFPexp ([]:fp_rw list) (e:exp) = e /\
+  rewriteFPexp ((lhs,rhs)::rwtl) e =
+    (case matchesFPexp lhs e [] of
+    |  SOME subst =>
+      (case appFPexp rhs subst of
+      | SOME e_opt => rewriteFPexp rwtl e_opt
+      | NONE => rewriteFPexp rwtl e)
+    | NONE => rewriteFPexp rwtl e)
+End
+
+Definition rewriteFPcexp_def:
+  rewriteFPcexp ([]:fp_rw list) (ce:exp) = ce /\
+  rewriteFPcexp ((lhs, rhs)::rwtl) ce =
+    (case matchesFPcexp lhs ce [] of
+      | SOME subst =>
+        (case appFPcexp rhs subst of
+          | SOME ce_opt => rewriteFPcexp rwtl ce_opt
+          | NONE => rewriteFPcexp rwtl ce)
+      | NONE => rewriteFPcexp rwtl ce)
+End
+
+Definition fp_add_comm_def:
+  fp_add_comm:fp_rw = (Binop FP_Add (Var 0) (Var 1), Binop FP_Add (Var 1) (Var 0))
+End
+
+val _ = export_theory();
